wip modular cut

Matroid/Constructions/ModularCut.lean
@@ -1,10 +1,15 @@
+import Matroid.ForMathlib.Order.Minimal
 import Matroid.Modular
 
 open Set Function Set.Notation
 
+variable {α : Type*} {M : Matroid α} {I J B F F' X Y : Set α} {e f : α}
+
+
+
 namespace Matroid
 
-variable {α : Type*} {M : Matroid α} {F F' X Y : Set α} {e f : α}
+
 
 structure ModularCut (M : Matroid α) where
   (carrier : Set (Set α))
@@ -42,6 +47,13 @@ lemma ModularCut.iInter_mem (U : M.ModularCut) {ι : Type*} [Nonempty ι] (Fs : 
   obtain ⟨B, hB, hB'⟩ := hFs_mod
   exact ⟨B, hB, by simpa⟩
 
+lemma ModularCut.inter_mem (U : M.ModularCut) (hF : F ∈ U) (hF' : F' ∈ U) (h : M.ModularPair F F') :
+    F ∩ F' ∈ U := by
+  rw [inter_eq_iInter]
+  apply U.iInter_mem
+  · simp [hF, hF']
+  exact h
+
 def ModularCut.Base (U : M.ModularCut) (e : α) (B : Set α) :=
   M.Base B ∨ (e ∈ B ∧ ∀ F ∈ U, ∃ f ∈ F, M.Base (insert f (B \ {e})))
 
@@ -55,51 +67,248 @@ def ModularCut.ConBase (U : M.ModularCut) (B : Set α) :=
   (M.Base B ∧ (U : Set (Set α)) = ∅) ∨
     ((U : Set (Set α)).Nonempty ∧ ∀ F ∈ U, ∃ f ∈ F, M.Base (insert f B))
 
-theorem ModularCut.conIndep_iff_subset_conBase (U : M.ModularCut)
-    {I : Set α} : U.ConIndep I ↔ ∃ B, U.ConBase B ∧ I ⊆ B := by
-
-  simp_rw [ModularCut.ConIndep, ModularCut.ConBase]
-  obtain (hU | hU) := (U : Set (Set α)).eq_empty_or_nonempty
-  · have h : ∀ F, F ∉ U := fun F (hF : F ∈ (U : Set (Set α))) ↦ by simp [hU] at hF
-    simp [h, hU, indep_iff]
-  simp only [hU.ne_empty, and_false, hU, true_and, false_or]
-  refine ⟨fun ⟨hI, hIU⟩ ↦ ?_, fun h ↦ ?_⟩
-  · obtain ⟨B, hB, hIB⟩ := hI.exists_base_superset
-    simp_rw [and_comm]
-    by_contra! hcon
-    -- rw [and_comm, not_exists] at hcon
-    -- have hx : ∀ x ∈ B \ I, ∃ F ∈ U, ∀ f ∈ F, ¬ M.Base (insert f (B \ {x})) :=
-    --   fun x hx ↦ hcon (B \ {x}) (subset_diff_singleton hIB hx.2)
-    have hdiff : ∀ x ∈ B \ I, M.cl (B \ {x}) ∈ U := by
-      intro x hx
-      obtain ⟨F, hFU, hF⟩ := hcon (B \ {x}) (subset_diff_singleton hIB hx.2)
-      refine U.cl_superset_mem hFU (fun f hf ↦ ?_)
-      rw [(hB.indep.diff {x}).mem_cl_iff', and_iff_right ((U.flat_of_mem hFU).subset_ground hf)]
-      have hfx : f ≠ x := by
-        rintro rfl; simpa [insert_eq_of_mem hx.1, hB] using hF f hf
-      rw [mem_diff, mem_singleton_iff, and_iff_left hfx]
-      exact fun hi ↦ by_contra fun hfB ↦ hF f hf <| hB.exchange_base_of_indep hfB hi
-    have _ : Nonempty ↑(B \ I) := by
-      rw [nonempty_iff_ne_empty', Ne, diff_eq_empty]; intro hBI
-      rw [hIB.antisymm hBI, hB.cl_eq] at hIU
-      obtain ⟨F, hF⟩ := hU
-      exact hIU <| U.superset_mem hF M.ground_flat (U.flat_of_mem hF).subset_ground
-
-    have h_inter := U.iInter_mem (Fs := fun x : ↑(B \ I) ↦ M.cl (B \ {x.1}))
-    simp only [Subtype.forall, iInter_coe_set, iff_true_intro hdiff, true_imp_iff] at h_inter
-    specialize h_inter ⟨B, hB, ?_⟩
-    · simp only [Subtype.forall, mem_diff, and_imp]
-      intro a haB haI
-      refine (hB.indep.inter_left _).basis_of_subset_of_subset_cl (inter_subset_left _ _)
-        (M.cl_subset_cl (subset_inter ?_ (diff_subset _ _)))
-      exact M.subset_cl _ ((diff_subset _ _).trans hB.subset_ground)
 
 
-    rw [biInter_eq_iInter, ← M.cl_iInter_eq_biInter_cl_of_iUnion_indep] at h_inter
-    · apply hIU
-      convert h_inter
-      ext x
-      simp
+
+
+    -- by_contra! hcon
+
+
+
+def ModularCut.ExtIndep (U : M.ModularCut) (e : α) (I : Set α) : Prop :=
+  (M.Indep I ∨ (M.Indep (I \ {e}) ∧ M.cl (I \ {e}) ∉ U))
+
+theorem ModularCut.ExtIndep.or {U : M.ModularCut} (hI : U.ExtIndep e I) (he : e ∉ M.E) :
+    (M.Indep I ∧ e ∉ I) ∨ (M.Indep (I \ {e}) ∧ M.cl (I \ {e}) ∉ U ∧ e ∈ I) := by
+  obtain (h | h) := hI
+  · exact .inl ⟨h, not_mem_subset h.subset_ground he⟩
+  obtain (heI | heI) := em (e ∈ I)
+  · exact .inr ⟨h.1, h.2, heI⟩
+  rw [diff_singleton_eq_self heI] at h
+  exact .inl ⟨h.1, heI⟩
+
+theorem ModularCut.ExtIndep.or' {U : M.ModularCut} (hI : U.ExtIndep e I) (he : e ∉ M.E) :
+    (M.Indep I ∧ e ∉ I) ∨ (∃ I₀, M.Indep I₀ ∧ M.cl I₀ ∉ U ∧ e ∉ I₀ ∧ I = insert e I₀) := sorry
+
+lemma ModularCut.extIndep_iff_of_mem {U : M.ModularCut} (he : e ∉ M.E) (heI : e ∈ I) :
+    U.ExtIndep e I ↔ (∃ I₀, M.Indep I₀ ∧ M.cl I₀ ∉ U ∧ e ∉ I₀ ∧ I = insert e I₀) := sorry
+
+lemma ModularCut.extIndep_iff_of_not_mem {U : M.ModularCut} (he : e ∉ M.E) (heI : e ∉ I) :
+    U.ExtIndep e I ↔ M.Indep I := sorry
+
+lemma ModularCut.ExtIndep.subset {U : M.ModularCut} (h : U.ExtIndep e I) (hJI : J ⊆ I) :
+    U.ExtIndep e J := by
+  sorry
+
+lemma ModularCut.extIndep_insert_iff {U : M.ModularCut} (he : e ∉ M.E) :
+    U.ExtIndep e (insert e I) ↔ M.Indep I ∧ M.cl I ∉ U := by
+sorry
+
+lemma ModularCut.ground_mem {U : M.ModularCut} (h : (U : Set (Set α)).Nonempty) : M.E ∈ U := sorry
+
+lemma ModularCut.ExtIndep.diff_singleton_indep {U : M.ModularCut} (h : U.ExtIndep e I) :
+    M.Indep (I \ {e}) := by
+  obtain (h | h) := h; exact h.diff _; exact h.1
+
+theorem ModularCut.extIndep_iff {U : M.ModularCut} (he : e ∉ M.E) :
+    U.ExtIndep e I ↔ (M.Indep I ∧ e ∉ I) ∨ (M.Indep (I \ {e}) ∧ M.cl (I \ {e}) ∉ U ∧ e ∈ I) := by
+  refine ⟨fun h ↦ h.or he, ?_⟩
+  rintro (h | h)
+  · exact .inl h.1
+  exact .inr ⟨h.1, h.2.1⟩
+
+def ModularCut.extendIndepMatroid (U : ModularCut M) (he : e ∉ M.E) : IndepMatroid α where
+
+  E := insert e M.E
+  Indep := U.ExtIndep e
+  indep_empty := Or.inl M.empty_indep
+  indep_subset _ _ := ModularCut.ExtIndep.subset
+
+
+
+    -- easy to fix
+    -- obtain (heI | heI) := em (e ∈ I)
+    -- · refine .inr ⟨hJ.1.subset (diff_subset_diff_left hIJ), fun hI ↦ hJ.2 ?_⟩
+    --   exact U.cl_superset_mem' hI (diff_subset_diff_left hIJ)
+    -- exact .inl (hJ.1.subset (subset_diff.2 ⟨hIJ, by simpa⟩))
+  indep_aug := by
+
+    rintro I B hI hInotmax hB
+    have ⟨hBi, hBins⟩ := (mem_maximals_iff_forall_insert (fun _ _ ↦ ExtIndep.subset)).1 hB
+    simp only [mem_maximals_iff, mem_setOf_eq, and_iff_right hBi] at hB
+    rw [mem_maximals_iff_forall_insert (fun _ _ ↦ ExtIndep.subset), and_iff_right hI] at hInotmax
+    push_neg at hInotmax
+
+
+    -- split into cases depending on why `B` is extension-independent.
+    obtain (⟨hBi, heB⟩ | ⟨B, hB, hBU, heB, rfl⟩) := hBi.or' he
+    · -- Case where `B` is a base of `M`.
+      replace hBi := hBi.base_of_maximal (fun J hJ ↦ hB (.inl hJ))
+
+      -- `I \ {e}` is not a base; if it were, we wouldn't have been able to extend `I`.
+      have hInb : ¬ M.Base (I \ {e}) := by
+        intro hIb
+        obtain ⟨x, hxI, hIx⟩ := hInotmax
+        obtain (rfl | hne) := eq_or_ne e x
+        · refine hBins e heB (.inr ⟨hBi.indep.subset (by simp), (fun hBU ↦ ?_)⟩)
+          rw [diff_singleton_eq_self hxI] at hIb
+          rw [U.extIndep_insert_iff he, hIb.cl_eq] at hIx
+          exact hIx.2 <| U.ground_mem ⟨_, hBU⟩
+
+        have hIex := (hIb.eq_of_subset_indep hIx.diff_singleton_indep
+          (diff_subset_diff_left (subset_insert _ _)))
+        rw [← insert_diff_singleton_comm hne.symm] at hIex
+        exact hxI (hIex.symm.subset <| .inl rfl).1
+
+      -- Therefore there is some `x ∈ B \ I` for which `I ∪ {x}` is independent.
+      obtain ⟨x, hx, hIx⟩ := hI.diff_singleton_indep.exists_insert_of_not_base hInb hBi
+      have hne : x ≠ e := by rintro rfl; simp [heB] at hx
+
+      -- Now split into cases depending on why `I` is extension-independent.
+      obtain (⟨hI, heI⟩ | ⟨I, hIi, hIU, heI, rfl⟩) := hI.or' he
+      · -- If `I` is independent, we win by augmenting using `x`.
+        exact ⟨x, by simpa [hne] using hx, .inl <| diff_singleton_eq_self heI ▸ hIx⟩
+
+      -- Otherwise, replace `I` with `I ∪ {e}` everywhere, where `I` is `M`-independent
+      -- and `M.cl I ∉ U`.
+      simp only [mem_singleton_iff, insert_diff_of_mem, diff_singleton_eq_self heI] at hIx
+
+      by_contra! hcon
+      simp_rw [mem_diff, mem_insert_iff, not_or, and_imp, insert_comm, extIndep_insert_iff he,
+        not_and, not_not] at hcon
+      replace hcon := fun x hx ↦ hcon x hx (by rintro rfl; contradiction)
+      have hxBI : x ∈ B \ I := by simpa [hne] using hx
+
+      -- If `I ∪ {x}` is a base, then since `I ∪ {e}` is not maximally extension-indep,
+      -- there is some `y` outside the span of `I` for which `cl (I ∪ {y}) ∉ U`.
+      -- But `cl (I ∪ {y}) = M.E = cl (I ∪ {x})`, so this contradicts the choice of `x`.
+      obtain (hIxb | hIxnb) := em (M.Base (insert x I))
+      · simp_rw [insert_comm, extIndep_insert_iff he, mem_insert_iff, not_or] at hInotmax
+        obtain ⟨y, ⟨hye, hyI⟩, hIy, hIyU⟩ := hInotmax
+        have hyxI : y ∉ insert x I := by
+          rintro (rfl | hyI)
+          · exact hIyU <| hcon y hx.1 hyI hIx
+          contradiction
+        have hyIb := hIxb.exchange_base_of_indep (e := x) (f := y) hyxI
+        simp only [mem_singleton_iff, insert_diff_of_mem, diff_singleton_eq_self hxBI.2, hIy,
+          true_implies] at hyIb
+        rw [hyIb.cl_eq, ← hIxb.cl_eq] at hIyU
+        exact hIyU <| hcon x hxBI.1 hxBI.2 hIx
+
+      -- If `I ∪ {x}` isn't a base, then there is some `y ∈ B` outside the span of `I ∪ {x}`.
+      -- But now (the closures of `I ∪ {x}` and `I ∪ {y}`) are a modular pair contained in `U`,
+      -- and we can contradict `cl I ∉ U`.
+      obtain ⟨y, hy, hyxI⟩ := hIx.exists_insert_of_not_base hIxnb hBi
+      simp only [mem_diff, mem_insert_iff, not_or] at hy
+      have hmod := U.inter_mem (hcon x hxBI.1 hxBI.2 hIx)
+        (hcon y hy.1 hy.2.2 (hyxI.subset (insert_subset_insert (subset_insert _ _)))) ?_
+      · rw [← Indep.cl_inter_eq_inter_cl, inter_insert_of_not_mem (by simpa using hy.2),
+          inter_eq_self_of_subset_right (subset_insert _ _)] at hmod
+        · contradiction
+        simpa [union_eq_self_of_subset_right (subset_insert _ _)]
+      apply ModularPair.cl_cl
+      apply Indep.modularPair_of_union
+      simpa [union_eq_self_of_subset_right (subset_insert _ _)]
+    rw [extIndep_insert_iff he] at hBi
+
+  -- Now consider the case where `B` has the form `B₀ ∪ {e}` with `B₀` independent and `cl B₀ ∉ U`.
+
+
+
+
+
+
+
+
+
+
+
+
+
+
+  indep_maximal := sorry
+  subset_ground := sorry
+
+
+      -- simp only [mem_diff, U.extIndep_iff he, mem_insert_iff, heI, or_true, not_true_eq_false,
+      --   and_false, and_true, false_or, not_and, not_not, and_imp] at hcon
+
+
+
+        -- have := U.cl_superset_mem' ?_ (show I ⊆ J \ {e} by sorry)
+
+
+      -- obtain (hI | hI) := hI
+      -- · -- `B` is a base and `I` is independent.
+
+
+
+      --   ·
+      --   -- have hI' : ¬ M.Base I := by
+      --   --   obtain ⟨J, (hJ | hJ), hIJ⟩ := hInotmax
+      --   --   · sorry --- easy
+
+
+      --   -- have := hI.exists_insert_of_not_base ?_ hB
+      -- sorry
+
+
+
+
+    -- obtain (hI | hI) := hI
+    -- · obtain ⟨(hB | hB), hBmax⟩ := hB
+    --   · -- case where `I,B` are independent.
+
+
+
+    -- rintro (hBi | ⟨hBi, hBU⟩) hI'
+    -- ·
+
+-- theorem ModularCut.conIndep_iff_subset_conBase (U : M.ModularCut)
+--     {I : Set α} : U.ConIndep I ↔ ∃ B, U.ConBase B ∧ I ⊆ B := by
+
+--   simp_rw [ModularCut.ConIndep, ModularCut.ConBase]
+--   obtain (hU | hU) := (U : Set (Set α)).eq_empty_or_nonempty
+--   · have h : ∀ F, F ∉ U := fun F (hF : F ∈ (U : Set (Set α))) ↦ by simp [hU] at hF
+--     simp [h, hU, indep_iff]
+--   simp only [hU.ne_empty, and_false, hU, true_and, false_or]
+--   refine ⟨fun ⟨hI, hIU⟩ ↦ ?_, fun h ↦ ?_⟩
+--   · obtain ⟨B, hB, hIB⟩ := hI.exists_base_superset
+--     simp_rw [and_comm]
+--     by_contra! hcon
+--     -- rw [and_comm, not_exists] at hcon
+--     -- have hx : ∀ x ∈ B \ I, ∃ F ∈ U, ∀ f ∈ F, ¬ M.Base (insert f (B \ {x})) :=
+--     --   fun x hx ↦ hcon (B \ {x}) (subset_diff_singleton hIB hx.2)
+--     have hdiff : ∀ x ∈ B \ I, M.cl (B \ {x}) ∈ U := by
+--       intro x hx
+--       obtain ⟨F, hFU, hF⟩ := hcon (B \ {x}) (subset_diff_singleton hIB hx.2)
+--       refine U.cl_superset_mem hFU (fun f hf ↦ ?_)
+--       rw [(hB.indep.diff {x}).mem_cl_iff', and_iff_right ((U.flat_of_mem hFU).subset_ground hf)]
+--       have hfx : f ≠ x := by
+--         rintro rfl; simpa [insert_eq_of_mem hx.1, hB] using hF f hf
+--       rw [mem_diff, mem_singleton_iff, and_iff_left hfx]
+--       exact fun hi ↦ by_contra fun hfB ↦ hF f hf <| hB.exchange_base_of_indep hfB hi
+--     have _ : Nonempty ↑(B \ I) := by
+--       rw [nonempty_iff_ne_empty', Ne, diff_eq_empty]; intro hBI
+--       rw [hIB.antisymm hBI, hB.cl_eq] at hIU
+--       obtain ⟨F, hF⟩ := hU
+--       exact hIU <| U.superset_mem hF M.ground_flat (U.flat_of_mem hF).subset_ground
+
+--     have h_inter := U.iInter_mem (Fs := fun x : ↑(B \ I) ↦ M.cl (B \ {x.1}))
+--     simp only [Subtype.forall, iInter_coe_set, iff_true_intro hdiff, true_imp_iff] at h_inter
+--     specialize h_inter ⟨B, hB, ?_⟩
+--     · simp only [Subtype.forall, mem_diff, and_imp]
+--       intro a haB haI
+--       refine (hB.indep.inter_left _).basis_of_subset_of_subset_cl (inter_subset_left _ _)
+--         (M.cl_subset_cl (subset_inter ?_ (diff_subset _ _)))
+--       exact M.subset_cl _ ((diff_subset _ _).trans hB.subset_ground)
+
+
+--     rw [biInter_eq_iInter, ← M.cl_iInter_eq_biInter_cl_of_iUnion_indep] at h_inter
+--     · apply hIU
+--       convert h_inter
+--       ext x
+--       simp
 
     -- rw [← M.cl_sInter_eq_biInter_cl_of_sUnion_indep] at h_inter
     -- have := M.cl_sInter_eq_biInter_cl_of_sUnion_indep
@@ -112,14 +321,14 @@ theorem ModularCut.conIndep_iff_subset_conBase (U : M.ModularCut)
 
 
 
-theorem ModularCut.indep_iff_subset_base (U : M.ModularCut) (he : e ∉ M.E) {I : Set α} :
-    U.Indep e I ↔ ∃ B, I ⊆ B ∧ U.Base e B := by
-  simp_rw [ModularCut.Indep, ModularCut.Base]
-  constructor
-  · rintro (hI | ⟨heI, hI, hIU⟩)
-    · obtain ⟨B, hB⟩ := hI.exists_base_superset
-      exact ⟨B, hB.2, .inl hB.1⟩
-    obtain ⟨B', hB', hIB'⟩ := hI.exists_base_superset
+-- theorem ModularCut.indep_iff_subset_base (U : M.ModularCut) (he : e ∉ M.E) {I : Set α} :
+--     U.Indep e I ↔ ∃ B, I ⊆ B ∧ U.Base e B := by
+--   simp_rw [ModularCut.Indep, ModularCut.Base]
+--   constructor
+--   · rintro (hI | ⟨heI, hI, hIU⟩)
+--     · obtain ⟨B, hB⟩ := hI.exists_base_superset
+--       exact ⟨B, hB.2, .inl hB.1⟩
+--     obtain ⟨B', hB', hIB'⟩ := hI.exists_base_superset
 
 
 
@@ -171,36 +380,3 @@ theorem ModularCut.indep_iff_subset_base (U : M.ModularCut) (he : e ∉ M.E) {I 
 
     -- have := hBmax (y := insert f (B \ {e}))
     -- rw [hB.mem_cl_iff]
-
-
-
-
-    -- by_contra! hcon
-
-
-
-
-
-def ModularCut.extendIndepMatroid (U : ModularCut M) (he : e ∉ M.E) : IndepMatroid α where
-  E := insert e M.E
-  Indep I := M.Indep I ∨ (M.Indep (I \ {e}) ∧ M.cl (I \ {e}) ∉ U)
-  indep_empty := Or.inl M.empty_indep
-  indep_subset := by
-    rintro I J (hJ | hJ) hIJ
-    · exact .inl <| hJ.subset hIJ
-    obtain (heI | heI) := em (e ∈ I)
-    · refine .inr ⟨hJ.1.subset (diff_subset_diff_left hIJ), fun hI ↦ hJ.2 ?_⟩
-      exact U.cl_superset_mem' hI (diff_subset_diff_left hIJ)
-    exact .inl (hJ.1.subset (subset_diff.2 ⟨hIJ, by simpa⟩))
-  indep_aug := by
-    rintro I B hI hInotmax hB
-    simp only [mem_maximals_iff, mem_setOf_eq] at hB
-    simp only [mem_maximals_iff, mem_setOf_eq, hI, true_and, not_forall, Classical.not_imp,
-      exists_prop, exists_and_left, and_assoc, ← ssubset_iff_subset_ne] at hInotmax
-    obtain ⟨J, hJ, hIJ⟩ := hInotmax
-    obtain ⟨x, hxJ, hxI⟩ := exists_of_ssubset hIJ
-
-    -- rintro (hBi | ⟨hBi, hBU⟩) hI'
-    -- ·
-  indep_maximal := _
-  subset_ground := _
